crc32

disk-betree/Framework.cs
@@ -380,5 +380,29 @@ namespace Crypto_Compile {
         return new Dafny.Sequence<byte>(hash);
       }
     }
+
+    public static Dafny.Sequence<byte> Crc32(Dafny.Sequence<byte> seq)
+    {
+      Native_Compile.BenchmarkingUtil.start();
+      using (var crc32 = DamienG.Security.Cryptography.Crc32.Create()) {
+        IList<byte> ilist = seq.Elements;
+        byte[] bytes = new byte[ilist.Count];
+        ilist.CopyTo(bytes, 0);
+
+        byte[] hash = crc32.ComputeHash(bytes);
+        Native_Compile.BenchmarkingUtil.end();
+
+				// Pad to 32 bytes
+				byte[] padded = new byte[32];
+				padded[0] = hash[0];
+				padded[1] = hash[1];
+				padded[2] = hash[2];
+				padded[3] = hash[3];
+				for (int i = 4; i < 32; i++) padded[i] = 0;
+
+        return new Dafny.Sequence<byte>(padded);
+      }
+    }
+
   }
 }
