lib/Crypto.s.dfy
@@ -5,4 +5,7 @@ module {:extern} Crypto {
 
   function method {:axiom} Sha256(t: seq<byte>) : (hash : seq<byte>)
   ensures |hash| == 32
+
+  function method {:axiom} Crc32(t: seq<byte>) : (hash : seq<byte>)
+  ensures |hash| == 32
 }
