Makefile
@@ -8,6 +8,6 @@ $(BUNDLE_SOURCE): $(shell find . -name '*.dfy')
 	mkdir -p build
 	dafny disk-betree/Bundle.i.dfy /spillTargetCode:3 /noVerify /compile:0 /out:build/Bundle.cs /countVerificationErrors:0
 
-FRAMEWORK_SOURCES=disk-betree/Framework.cs disk-betree/Benchmarks.cs
+FRAMEWORK_SOURCES=disk-betree/Framework.cs disk-betree/Benchmarks.cs disk-betree/Crc32.cs
 build/Veribetrfs.exe: $(FRAMEWORK_SOURCES) $(BUNDLE_SOURCE)
 	csc $(BUNDLE_SOURCE) $(FRAMEWORK_SOURCES) /r:System.Numerics.dll /debug /nowarn:0164 /nowarn:0219 /nowarn:1717 /nowarn:0162 /nowarn:0168 /out:build/Veribetrfs.exe
